### 2.5.7 

For a subgroup N of a group G, show that:  
#### a) $\Rightarrow$ b) Show that: $N$ is normal implies every left coset is a right coset

$N$ is normal, so $\forall g \in G,$ left coset $gN = gN(g^{-1}g) = (gNg^{-1})g = Ng$
which is a right coset. So all left cosets are right cosets.

#### b) $\Rightarrow$ c) Show that: Every left coset is a right coset implies $\forall a \in G, aN = Na$

We are given that $aN = Nb$.  
So, since $e \in N, \exists n' \in N: ae = n'b$  
$\Rightarrow ab^{-1} = n' \in N$   
So, by prop 30, $Aa = Ab = aA$

#### c) $\Rightarrow$ a) Show that: $\forall a \in G, aN = Na$ implies $N$ is normal

$$\begin{aligned}
aNa^{-1} &= (aN)a^{-1}                            \\
         &= (Na)a^{-1} \quad \text{since } aN = Na \\
         &= N
\end{aligned}$$
So $N$ is normal

---
### 2.5.13 (a) Show that the center of a group is a normal subgroup of $G$

Let $Z = Z(G) = \{ a \in G | ag = ga \forall g \in G \}$   

$$\begin{aligned}
\forall x \in G, xZx^{-1} &= \{ xzx^{-1} | \forall z \in Z \} \\
                          &=  \{ zxx^{-1} | \forall z \in Z \} \quad \text{
                          since z commutes with all elements of }G \\
                          &= \{z | \forall x \in Z \} \\
                          &= Z
\end{aligned}$$
So $Z(G)$ is normal

### 2.5.13 (b) What is the center of $S_3$

The center of $S_3$ is $\{e\}$ since, $S_3 \cong D_3 \equiv \langle a, r | a^2 =
e; r^3 = e; ra = ar^{-1} \rangle = \{e, r, r^2, a, ar, ar^2 \}$ and:
 * $a$ and $r$ do not commute: $ra = ar^{-1} = ar^2 \ne ar$
 * $a$ and $r^2$ do not commute: $r^2a = ar^{-2} = ar^4 = ar \ne ar^{2}$
 * $ar$ and $a$ do not commute: $ara = aar{^-1} = er^2 = r^2 \ne aar = r$
 * $ar^2$ and $r$ do not commute: $ar^2r = ae = a \ne rar^2 = ar^{-1}r^2 = ar$

---
### 2.6.1.

$f: X \to Y$ is surjective.

* $\forall x \in X, f(x) = f(x).$ So $\sim$ is reflexive.  
* $\forall x, y \in X, f(x) = f(y) \Rightarrow f(y) = f(x)$, so $x \sim y
  \Rightarrow y \sim x$: $\sim$ is symmetric.
* $\forall x, y, z \in X, f(x) = f(y) \text{ and } f(y) = f(z) \Rightarrow f(x) =
  f(z)$,  
  so $x\sim y$ and $y \sim z \Rightarrow x \sim z$

So $f$ is a equivalence relation.

---
### 2.7.9.

#### Show that $C$ is a normal subgroup

   $\forall c \in C, g\in G$,
   $$\begin{aligned}
      g^{-1}cg &= cc^{-1}g^{-1}cg \\
               &= c(c^{-1}g^{-1}cg) \\
               &= cc' \quad \text{where }c' \in C \\
      g^{-1}cg &\in C
   \end{aligned}
   $$
   So $C$ is a normal subgroup

#### Show that $G/C$ is abelian

   Let $a, b \in G$, then $aC, bC \in G/C$

   By def. of multiplication of quotient $aC\circ aB = abC$  
   But since $C$ is normal $bC = Cb$  
   So, $abC = aCb = Cab = abC$  
   So $G/C$ is abelian

#### $G/H$ is abelian  

   $$\begin{aligned}
   \forall a, b \in G, abH &= baH \\
                       a^{-1}b^{-1}abH &= H \\
                       a^{-1}b^{-1}ab &\in H
   \end{aligned}$$
   So, $H \supseteq C$

