---
title: Homework 13
---

### 5.4.1

**Given:** $|G| = p^3$, $p$ prime.  
**Show:** $|Z(G)| = p$ or $G$ is abelian.  

By Lagrage's theorem, $|Z(G)|$ must be one of $1, p, p^2, p^3$

By Prop 5.4.2, $|Z(G)|$ cannot be $1$

If $|Z(G)|$ is $p^2$, then $| G/Z(G) | = \frac {|G|}{|Z(G)|} = p$. So $G/Z(G)
\cong Z_p$. So by Ex. 2.7.11, $G$ must be abelian. But if $G$ is
abelian, then $Z(G) = G$, and $|Z(G)| = p^3$. This is a contradiction, so
$|Z(G)|$ cannot be $p^2$

If $|Z(G)|$ is $p^3$ then it contains all the elements of $|G|$ and $G$ must be
abelian.

So $|Z(G)|$ must be $p$ or $G$ must be abelian.

### 5.4.3

Given:
> $P$ is $p$-Sylow of $G$.  
> $H \le N_G(P)$  
> $|H| = p^s$

Show: $H \subseteq P$ 

5.4.11
6.1.5
6.1.6.
### 6.3.8

#### Show that $J[x]$ is an ideal of $R[x]$

* Non-empty: $J[x]$ not empty, since $0 \in J, \Rightarrow 0 \in J[x]$
* Abelian subgroup:
    - Closed under addition:
      for any $a = a_n x^n + \cdots + a_1 x + a_0, b = b_n x^n + \cdots + b_1 x + b_0 \in  J[x]$

      $$\begin{aligned}
          a + b &= (a_n x^n + \cdots + a_1 x + a_0) + (b_n x^n + \cdots + b_1 x + b_0) \\
                &= (a_n + b_n) x^n + \cdots + (a_1 + b+1) + (a_0 + b_0)
      \end{aligned}$$
      
      Since, $a_i, b_i \in J, (a_i + b_i) \in J \forall i$. So $a + b \in J[x]$
    - Inverses: Since $J$ is a field, $a_i \in J \Rightarrow -a_i \in J$. So $c = (-a_n x^n + \cdots + -a_1 x + -a_0) \in J[x]$
      $$\begin{aligned}
          a + c &= (a_n x^n + \cdots + a_1 x + a_0) + (-a_n x^n + \cdots + -a_1 x + -a_0) \\
                &= (a_n + -a_n) x^n + \cdots + (a_1 + -a_1) + (a_0 + -a_0) \\
                &= 0
      \end{aligned}$$
      So $c = -a$ and every element in $J[x]$ has an inverse.
    - Since $J[x]$ is a ring, addition commutes
* $\forall j \in J[x], r \in R[x]$
  $$\begin{aligned}
      a \cdot b &= (\sum_{m=0}^M j_m x^m) (\sum_{n=0}^N r_n x^n) \\
                &= \sum_{m=0}^M \sum_{n=0}^N (j_m x^m) ( r_n x^n) \\
                &= \sum_{m=0}^M \sum_{n=0}^N (j_m r_n x^{m+n}) \\
  \end{aligned}$$
  Since $J$ is an ideal of $R$, $j_m r_n \in J$, and $a \cdot b = \sum_{m=0}^M \sum_{n=0}^N (j_m r_n x^{m+n}) \in J[x]$

---
#### Show that $R[x]/J[x] \cong (R/J)[x]$

Let $\varphi: R[x]/J[x] \to (R/J)[x]$,  
$\varphi(r J[x]) = \sum_{n=0}^N r_nJ x^n$  
Then, $\forall XXX$...

$$\begin{aligned}
\varphi((a J[x]) + (b J[x])) &= \varphi((a+b) J[x]) \\
                             &= \sum_{n=0}^N (a_n + b_n)J x^n  \\
                             &= \sum_{n=0}^N a_n J x^n + b_n J x^n \\
                             &= \sum_{n=0}^N a_n J x^n + \sum_{n=0}^N b_n J x^n  \\
                             &= \varphi(aJ[x]) + \varphi(bJ[x])
\end{aligned}$$

and,

$$\begin{aligned}
\varphi((a J[x])(b J[x])) &= \varphi((a\cdot b) J[x]) \\
                          &= \varphi((\sum_{i=0}^N \sum_{j=0}^N (a_i x^i) ( b_j x^j) ) J[x]) \\
                          &= \sum_{i=0}^N \sum_{j=0}^N \varphi((a_i x^i) ( b_j x^j) J[x] )\\
                          &= \sum_{i=0}^N \sum_{j=0}^N \varphi((a_i b_j x^{i+j}) J[x] )\\
                          &= \sum_{i=0}^N \sum_{j=0}^N (a_i b_j) J x^{i+j} \\
                          &= \sum_{i=0}^N \sum_{j=0}^N (a_i J x^i)(b_j J x^j) \\
                          &= \sum_{i=0}^N (a_i J x^i)\sum_{j=0}^N (b_j J x^j) \\
                          &= \varphi(aJ[x])\varphi(bJ[x])
\end{aligned}$$

For all $aJ[x] = (\sum_{n=0}^N a_n x^n)J[x] \in R[x]/J[x]$, there is a $\sum_{n=0}^N a_n J x^n \in (R/J)[x]$. So $\varphi$ is surjective.

Let $a = \sum_{n=0}^N a_n J x^n$, $b = \sum_{n=0}^N b_n J x^n$ and $\varphi(a) =
\varphi(b)$.
