Theorem  6.11.  Let  V  be  an  inner  product   space,  and  let  T  and  U  be
linear  operators  on  V.   Then
show  (cT)*  =  \bar eT*  for any  c \in  F; 

2(c)

g(f) = f(0) + f'(1) \\
     = f(0)


3(b)

$$\begin{aligned}
<T(x), y> &= 
\end{aligned}$$


3(c)

f(t) = at + b
f'(t) = a
f(t) = f'(t)t + b
f'(t)t = f(t) - b


$$\begin{aligned}
<T(f), g> &= \int_{-1}^1 (T(f)(t))g(t) dt \\
          &= \int_{-1}^1 (f'(t) + 3f(t))g(t) dt \\
          &= \int_{-1}^1 (f'(t) + 3f(t))g(t) dt \\
          &= \int_{-1}^1 f'(t)g(t) + 3f(t)g(t) dt \\
          &= \int_{-1}^1 f'(t)g(t) + 3f(t)g(t) dt \\
          &= \int_{-1}^1 f'(t)g(t) + 3f(t)g(t) dt \\
\end{aligned}$$
