\newcommand M22 = {M_{2\times 2}}

1.  $\Q$'s field of fractions is $\Z$. By Gauss' lemma, each of these
    are reducible in $\Q[x]$ iff they are reducible in $\Z[x]$.

    $2\Z$ is a proper ideal of $\Z$.

    a.  $x^4 - 3x + 9$. In $\Z/2Z$, $x^4 +x + 1$ has no roots and so no
        factors of degree 1 and 3.

        This leaves the polynomials of degree two: $x^2 + x$, $x^2$,
        $x^2 + x + 1$ and $x^2 + 1$. The first two are reducible into
        two polynomials of degree 1.
        
        But, $$\begin{aligned}
           (x^2 + x + 1) ( x^2 + x + 1) 
               &= x^4 + x^3 + x^2 + x^3 + x^2 + x + x^2 + x + 1 
               &= x^4 + x^2 + 1 \\
           (x^2 + x + 1) ( x^2 + 1) 
               &= x^4 + x^3 + x^2 + x^2 + x + 1 
               &= x^4 + x^3 + 1 \\
           (x^2 + 1) ( x^2 + 1) 
               &= x^4 + x^2 + x^2 +  1 
               &= x^4 + 1 \\
        \end{aligned}$$
        
        So, since the polynomial $f(x)/(2)$ is not factorizable, $f(x)$
        is not factorizable either, in both $\Z[x]$ and $\Q[x]$.

    b.  $f(x) = x^4 -9 x^2 + 3$: Let $P = (3)$, prime in $\Z$.
        $3 \notin P^2$ and $3, -9 \in P$. By Eisenstien's criteria,
        $f(x)$ is irreducible in $\Z[x]$ and so in $\Q[x]$.

    c.  $f(x) = x^4 - 3x^2 + 9 = (x^2 - 3x + 3)(x^2 +3x + 3)$:

2.  a.  Let $\phi: S \times N \to l$, $\phi: (s, n) \mapsto s\phi(n)$.

        $\phi$ is a map on sets from $S \times N \to L$, and $L$ is an
        $R-$module. By theorem 6, there exists a (unique) free $R-$
        module $F(S \times N)$ on $S\times N$ such that for any
        $R-$module, $\Phi(a) = \phi(a)$.

    b.  Assume $s, s_1, s_2 \in S$ and $n, n_1, n_2 \in N$.
        i.e. they are in the generating set of the free submodule.
    
        $$\begin{aligned}
         &\Phi((s, n_1 + n_2) - (s, n_1) - (s, n_2))                \\
        =&\Phi((s, n_1 + n_2)) - \Phi((s, n_1)) - \Phi((s, n_2))    \\
        =&\phi((s, n_1 + n_2)) - \phi((s, n_1)) - \phi((s, n_2))    \\
        =&s\phi(n_1 + n_2) - s\phi(n_1) - s\phi(n_2)                \\
        =&s \phi(n_1 + n_2) - \phi(n_1) - \phi(n_2)                 \\
        =&s \phi(n_1 + n_2  -      n_1  -      n_2)                 \\
        =&s \phi(0)                                                 \\
        =&s 0                                                       \\
        \end{aligned}$$
        
        $$\begin{aligned}
            \Phi(   (s_1 + s_2, n)  - (s_1, n)  - (s_2, n)  )       \\
        =&  \Phi((s_1 + s_2, n)) - \Phi((s_1, n)) - \Phi((s_2, n))  \\
        =&  (s_1 + s_2)\phi(n) - s_1\phi(n) - s_2\phi(n)            \\
        =&  (s_1 + s_2 - s_1 - s_2) \phi(n)                         \\
        =& 0 \phi(n) = 0
        \end{aligned}$$

        $$\begin{aligned}
           \Phi(   (rs, n) - (s, rn))      \\
        =& \Phi((rs, n)) - \Phi((s, rn))      \\
        =& \phi((rs, n)) - \phi((s, rn))      \\
        =& rs\phi(n) - s\phi(rn)      \\
        =& rs\phi(n) - sr\phi(n)      \\
        =  0 
        \end{aligned}$$
        
    c.   

3.  a.  Since $\Q$ is a field, $R$ is an euclidian domain and a PID.

        Let $I \subset I_1 \subset I_2 \cdots \subset$ be an ascending
        chain of ideals. Assume that this chain doesn't stabilize. Then,
        there is some $I_i \ne I_j \ne 0, i < j$ in the chain. Let
        $x \in I_i$. and $y \in I_j$. Since $R$ is a PID,
        $x = p_1 p_2 p_3 \ldots p_n$.

        Then $I_i = (a) = (p_1 p_2 \ldots p_n)$,
        $p_1, p_2, \ldots, p_n$\
        prime in $R$, since $R$ is a PID.

        Similarly $I_j = (b)$. But since $a \in (b), \gcd(a, b) = b$ and
        $b | a$. This means that $b$'s prime factorization is a subset
        of $a$'s and that by induction, must become $(1) = R$ and
        stabalize.

    b.  $R \supset (x) \supset (x^2) \supset (x^4) \supset \cdots$.
   
