---
title: Math 500 - Homework 6
---

1.  a.  Let $R$ be a UFD. Show that every nonzero prime ideal $I$ in $R$
        contains an irreducible element $x$. 
    
    
        Let $I$ be a prime ideal, then $a \ne 0 \in I \implies a = p_1 \cdots p_n$,
        for some irreducibles $p_1, \ldots p_n$.
        But since $I$ is prime, either $p_1 \in I$ and we are done, or $p_2 \cdots p_n \in I$.
        Since $n$ is finite, there must be some $p_i \in I$.
       
        
    b.  Let $P \ne 0$ prime in $R$. $P$ maximal. 
    
    
        By `1 (a)` there is some irreducible element $x \in P$.
        $(x) \subseteq P$. But by assumption $(x)$ is maximal, and $P = R$ or
        $P = (x)$. But $P = R \implies P = (1)$. So $P$ is principle.
    
    
2.  Let $h: M_1 \oplus M_2 \to (M_1 / N_1 ) \oplus (M_2 / N_2 )$,
	$h: (m_1 , m_2 ) \mapsto (m_1 + N_1, m_2 + N_2)$.

    *   Show that $h$ is a homomorphism:

        Let $(m_1, m_2), (m_1', m_2') \in M_1 \oplus M_2$.
        Then $h((m_1, m_2) + (m_1', m_2')) = h((m_1 + m_1', m_2 + m_2'))
                                           = (m_1 + m_1' + N_1, m_2 + m_2' + N_2)
                                           = (m_1 + N_1, m_2 + N_2) + (m_1' + N_1, m_2' + N_2)
                                           = h(m_1, m_2) + h(m_1', m_2')$.

    *   Show that $\ker(h) = N_1 \oplus N_2$

        Let $(m_1, m_2) \in \ker(h)
        \iff h(m_1, m_2) = (m_1 + N_1, m_2 + N_2) = (N_1, N_2)
        \iff m_1 \in N_1, m_2 \in N_2$
        
    By the first isomorphism theorem, $\frac {M_1 \oplus M_2 }{N_1 \oplus N_2} \cong M_1 / N_1 \oplus M_2 / N_2$

3.  Let $a(x) = \sum_{i<8} a_i x^i \in M$. Then let
    $8a(x) = (a(x)^8)  = { \sum_{i<8} a_i x^{i} }^8 = \sum_{i<8} b_i x^{i}$.
    -   $b_0 = 1^8 = 1$.
    -   $b_1 = \binom 8 1 a_1 = 8 a_1 = 0$
    -   $b_2 = \binom 8 2 a_1 + \binom 8 1 a_2 = 28 a_1 + 8 a_2 = 0$
    -   ...

    i.e. forall $8a(x), 8a(x) = 0$ and
    $8 \in \ann(M) \implies (8) \subseteq \ann(M)$.

    Since $\ann(M) \subset \Z$, $\ann(M) \in \{ (1), (2), (4), (8) \}$.
    But
    -   $\ann(M) \ne (1)$, since $(x + 1)^1 \ne 1$
    -   $\ann(M) \ne (2)$, since $(x + 1)^2 = x^2 + 1 \ne 1$
    -   $\ann(M) \ne (4)$, since
        $(x + 1)^4 = (x^2 + 1)^2 = x^4 + 1 \ne 1$

4.  $$
    \begin{aligned}
        &\begin{bmatrix}
        x-1     & 1     & 1 \\
        0       & x-2   & 1 \\
        0       & 0     & x - 1\\
        \end{bmatrix} 
    \to \begin{bmatrix}
        x-1     & x     & 1 \\
        0       & x-2   & 1 \\
        0       & 0     & x - 1\\
        \end{bmatrix} 
    \to \begin{bmatrix}
         -1     & x     & 1 \\
        -x+ 2   & x-2   & 1 \\
        0       & 0     & x - 1\\
        \end{bmatrix} 
    \to \begin{bmatrix}
         -1     & x     & 1 \\
        0       & (x-2)(1 - x)   & x - 3 \\
        0       & 0     & x - 1\\
        \end{bmatrix} \\ 
    \to & \begin{bmatrix}
         -1     & 0     & 1 \\
        0       & (x-2)(1 - x)   & x - 3 \\
        0       & 0     & x - 1\\
        \end{bmatrix} 
    \to \begin{bmatrix}
         -1     & 0     & 1 \\
        0       & (x-2)(1 - x)   & -2 \\
        0       & 0     & x - 1\\
       \end{bmatrix} 
    \to \begin{bmatrix}
         -1     & 0     & 1 \\
        -2       & (x-2)(1 - x)   & 0 \\
        0       & 0     & x - 1\\
        \end{bmatrix}  \\
    \to & \begin{bmatrix} 
         -1     & 0     & 0 \\
        -2       & (x-2)(1 - x)   & 0 \\
        0       & 0     & x - 1\\
        \end{bmatrix} 
    \to  \begin{bmatrix}
         -1     & 0     & 0 \\
        0       & (x-2)(1 - x)   & 0 \\
        0       & 0     & x - 1\\
        \end{bmatrix} 
    \to \begin{bmatrix}
         1     & 0     & 0 \\
        0       & x -1    & 0 \\
        0       & 0     & (x - 1)(x - 2)\\
        \end{bmatrix} 
    \end{aligned}
    $$
    The required invariant factors are $x -1 , (x-1)(x-2)$
    
    
5.  $$\begin{aligned}
    & \begin{bmatrix}
        2 &     2 &     3 \\
        2 &     8 &     2 \\
        4 &     4 &     1 \\
        \end{bmatrix}
    \to \begin{bmatrix}
        4 &     4 &     1 \\
        2 &     8 &     2 \\
        2 &     2 &     3 \\
        \end{bmatrix}
    \to \begin{bmatrix}
        1 &     4 &     4 \\
        2 &     8 &     2 \\
        3 &     2 &     2 \\
        \end{bmatrix}
    \to \begin{bmatrix}
        1 &     4 &     4 \\
        0 &     0 &    -6 \\
        0 &   -10 &   -10 \\
        \end{bmatrix}
    \to \begin{bmatrix}
        1 &     0 &     4 \\
        0 &     6 &    -6 \\
        0 &     0 &   -10 \\
        \end{bmatrix} \\
    \to &\begin{bmatrix}
        1 &     0 &     4 \\
        0 &     6 &    -6 \\
        0 &     0 &   -10 \\
        \end{bmatrix}
    \to \begin{bmatrix}
        1 &     0 &     4 \\
        0 &     6 &    -6 \\
        0 &    -6 &    -4 \\
        \end{bmatrix}
    \to \begin{bmatrix}
        1 &     0 &     4 \\
        0 &    12 &    -2 \\
        0 &    -6 &    -4 \\
        \end{bmatrix}
    \to \begin{bmatrix}
        1 &     0 &     4 \\
        0 &    12 &    -2 \\
        0 &     6 &     4 \\
        \end{bmatrix}
    \to \begin{bmatrix}
        1 &     0 &     4 \\
        0 &    12 &    -2 \\
        0 &     6 &     4 \\
        \end{bmatrix} \\
    \to & \begin{bmatrix}
        1 &     0 &     4 \\
        0 &    12 &    -2 \\
        0 &    30 &     0 \\
        \end{bmatrix}
    \to \begin{bmatrix}
        1 &     0 &     4 \\
        0 &     0 &    -2 \\
        0 &    30 &     0 \\
        \end{bmatrix}
    \to \begin{bmatrix}
        1 &     0 &     0 \\
        0 &     0 &    -2 \\
        0 &    30 &     0 \\
        \end{bmatrix}
    \to \begin{bmatrix}
        1 &     0 &     0 \\
        0 &     2 &     0 \\
        0 &     0 &    30 \\
        \end{bmatrix}
    \end{aligned}$$

    The invariant factors are 2, and 18
    
    
    
