---
title: Homework 9 - CS 476
---

ITP
===

First, we load the `ITP` tool:

```{ pipe="tee root/prove-commutativity.maude " }
load nat-au.maude
load itp-tool.maude
loop init-itp .

```


Given the module:

```{ pipe="tee nat-au.maude" }
fmod NAT-AU is
    sort Nat* .
    op 0   :           -> Nat* [ctor] .
    op 1   :           -> Nat* [ctor] .
    op _+_ : Nat* Nat* -> Nat* [ctor assoc id: 0] .
endfm

```

we prove:

```{ pipe="tee -a root/prove-commutativity.maude" }
(goal commutative : NAT-AU |- A{ X:Nat* ; Y:Nat* } ((X + Y) = (Y + X)) . )

```

as follows:

```{ pipe="tee -a root/prove-commutativity.maude" }
(cns X .)
(ind on Y .)
    
    (auto .)
    
    (lem one-commutes : A{ X:Nat* } ((X + 1) = (1 + X)) .)  
    (ind* on X .)
    (a-inst lem-one-commutes with (X:Nat* <- X*Nat*) .)   
    (disable lem-one-commutes .)
    (auto .)
        
    (auto .)
```

<!--
```
load nat-au.maude
load itp-tool.maude
loop init-itp .

(goal commutative : NAT-AU |- A{ X:Nat* ; Y:Nat* } ((X + Y) = (Y + X)) . )
(ind on Y:Nat* .)

    (auto .)
    
    (ind on X .)
    
        (auto .)
        
        (auto .)
        
        (cns .)            
        (imp .)
        (disable hyp-0 .)
        (auto .)
        (enable hyp-0 .)
        (disable hyp-1 .)
        (auto .)
        
    (cns .)
    (imp .)
    (cns .)
    (a-inst hyp-0 with (X:Nat* <- X*Nat*) . )
    (a-inst hyp-1 with (X:Nat* <- X*Nat*) . )
    (disable hyp-0 .)
    (disable hyp-1 .)
    (auto .)
```
-->

This outputs:

```{ pipe="maude -no-banner root/prove-commutativity.maude 2>&1" }
```

2
====

\newcommand \Alg {\mathcal T}
\newcommand \sme {\Sigma / E}
\newcommand \smp {\Sigma / E'}
\newcommand \smg {\Sigma / G}
\newcommand \equalsE {=_E}
\newcommand \equalsG {=_{E\union G}}

1.
    Let $t =_{E\union G} t'$. Then there is a proof
    $t = t_1 \equalsG t_2 \equalsG \ldots \equalsG t_n = t'$. If every
    $t_i \equalsE t_{i+1} \in E$, then this is a valid $E-$proof. Otherwise,
    there is some $i$ where $t_i \equalsE t_{i+1} \notin E, \in G$. Since
    $E \satisfies G$, $E \proves G$, and we can replace that proof step with
    an $E-$proof. This the equivalence classes mod $E$ and mod $E\union G$
    are the same. By initiality, there is a unique $\Sigma$ algebra on this
    set, and the algebras must be the same.

2.  Yes, they are isomorphic. In `1.` we showed that `NAT-AU` $\proves$ `comm`, by
    soundness `NAT-AU` $\satisfies$ `comm`, by `2.1.`, `NAT-AU` $\iso$ `NAT-ACU`.

3.  Let $i$ be the isomorphism between $\Alg_\sme$ and $\Alg_\smp$
    are both $\Sigma-$algebras. Let $g$ and $h$
    resp. be the unique isomorphism from $\Alg_\Sigma$ to each. Let $t$ be a
    term in $\Alg_\Sigma$, then $g(t) = [t]_E$. By initiallity,
    $g(t) = i(h(t)) \implies [t]_E = i([t]_{E'}$. So
    $\forall t, t' \in \Alg_\Sigma, t' \in [t]_{E'} \iff t' \in [t]_{E}$.
    By completeness, $E \proves t = t' \iff E' \proves t = t'$ and $E \equiv E'$.


    Alternate proof (input from Aditya): By definition,
    $\Alg_\sme \satisfies E$, but
    $\Alg_\smp \cong \Alg_\sme \implies \Alg_\smp \satisfies E$. By
    completeness, $\Alg_\smp \proves E$. By symmetry, $\Alg_\sme \proves E'$
    and $(\Sigma, E ) \equiv (\Sigma, E')$.

---


`a-inst`:
:   The `a-inst` command lets you instantiate a universally quantified
    equation with something more specific. This is useful for building a
    terminating set of equations after new hypothesis have been added
    via `lem` or `imp`.

    The syntax for `a-inst` is `( a-inst Label with Substitution .)`
    where `Substitution` is a "`;`"-separated list of `Assignement`s.
    Each assignment is of the for `Variable <- Term`.

    For example, given the equation,
    `eq X:Nat* + Y:Nat* = Y:Nat* + X:Nat*  [ label comm ] .`, running
    `(a-inst comm with (X:Nat* <- 1) .)` will add a new equation
    `eq 1 + Y:Nat* = Y:Nat* + 1 [...] .`.

`show-all`:
:   Lists out all `eq`s and `op`s of the module (including new
    hypothesis added by `imp` and `lem`).
